dotprod.v
@@ -6,29 +6,20 @@ Local Open Scope string_scope.
 Local Open Scope clight_scope.
 
 Module Info.
-  Definition version := "3.10".
+  Definition version := "3.11".
   Definition build_number := "".
   Definition build_tag := "".
   Definition build_branch := "".
   Definition arch := "x86".
-  Definition model := "32sse2".
+  Definition model := "64".
   Definition abi := "standard".
-  Definition bitsize := 32.
+  Definition bitsize := 64.
   Definition big_endian := false.
   Definition source_file := "dotprod.c".
   Definition normalized := true.
 End Info.
 
-Definition _N : ident := $"N".
-Definition _R : ident := $"R".
-Definition _REPEAT : ident := $"REPEAT".
 Definition _T : ident := $"T".
-Definition __155 : ident := $"_155".
-Definition __156 : ident := $"_156".
-Definition __229 : ident := $"_229".
-Definition __230 : ident := $"_230".
-Definition __231 : ident := $"_231".
-Definition __Bigint : ident := $"_Bigint".
 Definition ___builtin_annot : ident := $"__builtin_annot".
 Definition ___builtin_annot_intval : ident := $"__builtin_annot_intval".
 Definition ___builtin_bswap : ident := $"__builtin_bswap".
@@ -65,7 +56,6 @@ Definition ___builtin_va_end : ident := $"__builtin_va_end".
 Definition ___builtin_va_start : ident := $"__builtin_va_start".
 Definition ___builtin_write16_reversed : ident := $"__builtin_write16_reversed".
 Definition ___builtin_write32_reversed : ident := $"__builtin_write32_reversed".
-Definition ___cleanup : ident := $"__cleanup".
 Definition ___compcert_i64_dtos : ident := $"__compcert_i64_dtos".
 Definition ___compcert_i64_dtou : ident := $"__compcert_i64_dtou".
 Definition ___compcert_i64_sar : ident := $"__compcert_i64_sar".
@@ -85,155 +75,27 @@ Definition ___compcert_va_composite : ident := $"__compcert_va_composite".
 Definition ___compcert_va_float64 : ident := $"__compcert_va_float64".
 Definition ___compcert_va_int32 : ident := $"__compcert_va_int32".
 Definition ___compcert_va_int64 : ident := $"__compcert_va_int64".
-Definition ___count : ident := $"__count".
-Definition ___getreent : ident := $"__getreent".
-Definition ___locale_t : ident := $"__locale_t".
-Definition ___sFILE64 : ident := $"__sFILE64".
-Definition ___sbuf : ident := $"__sbuf".
-Definition ___sdidinit : ident := $"__sdidinit".
-Definition ___sf : ident := $"__sf".
-Definition ___sglue : ident := $"__sglue".
-Definition ___stringlit_1 : ident := $"__stringlit_1".
-Definition ___stringlit_2 : ident := $"__stringlit_2".
-Definition ___tm : ident := $"__tm".
-Definition ___tm_hour : ident := $"__tm_hour".
-Definition ___tm_isdst : ident := $"__tm_isdst".
-Definition ___tm_mday : ident := $"__tm_mday".
-Definition ___tm_min : ident := $"__tm_min".
-Definition ___tm_mon : ident := $"__tm_mon".
-Definition ___tm_sec : ident := $"__tm_sec".
-Definition ___tm_wday : ident := $"__tm_wday".
-Definition ___tm_yday : ident := $"__tm_yday".
-Definition ___tm_year : ident := $"__tm_year".
-Definition ___value : ident := $"__value".
-Definition ___wch : ident := $"__wch".
-Definition ___wchb : ident := $"__wchb".
-Definition __add : ident := $"_add".
-Definition __asctime_buf : ident := $"_asctime_buf".
-Definition __atexit : ident := $"_atexit".
-Definition __atexit0 : ident := $"_atexit0".
-Definition __base : ident := $"_base".
-Definition __bf : ident := $"_bf".
-Definition __blksize : ident := $"_blksize".
-Definition __close : ident := $"_close".
-Definition __cookie : ident := $"_cookie".
-Definition __cvtbuf : ident := $"_cvtbuf".
-Definition __cvtlen : ident := $"_cvtlen".
-Definition __data : ident := $"_data".
-Definition __dso_handle : ident := $"_dso_handle".
-Definition __emergency : ident := $"_emergency".
-Definition __errno : ident := $"_errno".
-Definition __file : ident := $"_file".
-Definition __flags : ident := $"_flags".
-Definition __flags2 : ident := $"_flags2".
-Definition __fnargs : ident := $"_fnargs".
-Definition __fns : ident := $"_fns".
-Definition __fntypes : ident := $"_fntypes".
-Definition __freelist : ident := $"_freelist".
-Definition __gamma_signgam : ident := $"_gamma_signgam".
-Definition __getdate_err : ident := $"_getdate_err".
-Definition __glue : ident := $"_glue".
-Definition __h_errno : ident := $"_h_errno".
-Definition __inc : ident := $"_inc".
-Definition __ind : ident := $"_ind".
-Definition __iobs : ident := $"_iobs".
-Definition __is_cxa : ident := $"_is_cxa".
-Definition __k : ident := $"_k".
-Definition __l64a_buf : ident := $"_l64a_buf".
-Definition __lb : ident := $"_lb".
-Definition __lbfsize : ident := $"_lbfsize".
-Definition __locale : ident := $"_locale".
-Definition __localtime_buf : ident := $"_localtime_buf".
-Definition __lock : ident := $"_lock".
-Definition __maxwds : ident := $"_maxwds".
-Definition __mblen_state : ident := $"_mblen_state".
-Definition __mbrlen_state : ident := $"_mbrlen_state".
-Definition __mbrtowc_state : ident := $"_mbrtowc_state".
-Definition __mbsrtowcs_state : ident := $"_mbsrtowcs_state".
-Definition __mbstate : ident := $"_mbstate".
-Definition __mbtowc_state : ident := $"_mbtowc_state".
-Definition __mult : ident := $"_mult".
-Definition __nbuf : ident := $"_nbuf".
-Definition __new : ident := $"_new".
-Definition __next : ident := $"_next".
-Definition __nextf : ident := $"_nextf".
-Definition __niobs : ident := $"_niobs".
-Definition __nmalloc : ident := $"_nmalloc".
-Definition __offset : ident := $"_offset".
-Definition __on_exit_args : ident := $"_on_exit_args".
-Definition __p : ident := $"_p".
-Definition __p5s : ident := $"_p5s".
-Definition __r : ident := $"_r".
-Definition __r48 : ident := $"_r48".
-Definition __rand48 : ident := $"_rand48".
-Definition __rand_next : ident := $"_rand_next".
-Definition __read : ident := $"_read".
-Definition __reent : ident := $"_reent".
-Definition __result : ident := $"_result".
-Definition __result_k : ident := $"_result_k".
-Definition __seed : ident := $"_seed".
-Definition __seek : ident := $"_seek".
-Definition __seek64 : ident := $"_seek64".
-Definition __sig_func : ident := $"_sig_func".
-Definition __sign : ident := $"_sign".
-Definition __signal_buf : ident := $"_signal_buf".
-Definition __size : ident := $"_size".
-Definition __stderr : ident := $"_stderr".
-Definition __stdin : ident := $"_stdin".
-Definition __stdout : ident := $"_stdout".
-Definition __strtok_last : ident := $"_strtok_last".
-Definition __ub : ident := $"_ub".
-Definition __ubuf : ident := $"_ubuf".
-Definition __unspecified_locale_info : ident := $"_unspecified_locale_info".
-Definition __unused : ident := $"_unused".
-Definition __unused_rand : ident := $"_unused_rand".
-Definition __up : ident := $"_up".
-Definition __ur : ident := $"_ur".
-Definition __w : ident := $"_w".
-Definition __wcrtomb_state : ident := $"_wcrtomb_state".
-Definition __wcsrtombs_state : ident := $"_wcsrtombs_state".
-Definition __wctomb_state : ident := $"_wctomb_state".
-Definition __wds : ident := $"_wds".
-Definition __write : ident := $"_write".
-Definition __x : ident := $"_x".
-Definition _acquire : ident := $"acquire".
-Definition _argc : ident := $"argc".
-Definition _argv : ident := $"argv".
-Definition _atoi : ident := $"atoi".
-Definition _atom_int : ident := $"atom_int".
 Definition _closure : ident := $"closure".
-Definition _d : ident := $"d".
 Definition _delta : ident := $"delta".
 Definition _delta_next : ident := $"delta_next".
-Definition _delta_next__1 : ident := $"delta_next__1".
 Definition _do_tasks : ident := $"do_tasks".
 Definition _dotprod : ident := $"dotprod".
 Definition _dotprod_task : ident := $"dotprod_task".
 Definition _dotprod_worker : ident := $"dotprod_worker".
 Definition _dtasks : ident := $"dtasks".
-Definition _exit : ident := $"exit".
-Definition _fprintf : ident := $"fprintf".
-Definition _freelock : ident := $"freelock".
-Definition _goal : ident := $"goal".
+Definition _exit_thread : ident := $"exit_thread".
 Definition _i : ident := $"i".
 Definition _initialize_task : ident := $"initialize_task".
-Definition _j : ident := $"j".
 Definition _main : ident := $"main".
 Definition _make_dotprod_tasks : ident := $"make_dotprod_tasks".
 Definition _make_tasks : ident := $"make_tasks".
-Definition _makelock : ident := $"makelock".
 Definition _malloc : ident := $"malloc".
 Definition _n : ident := $"n".
 Definition _num_threads : ident := $"num_threads".
-Definition _placeholder : ident := $"placeholder".
-Definition _printf : ident := $"printf".
-Definition _release : ident := $"release".
 Definition _result : ident := $"result".
-Definition _spawn : ident := $"spawn".
 Definition _t : ident := $"t".
 Definition _task : ident := $"task".
 Definition _tasks : ident := $"tasks".
-Definition _test : ident := $"test".
 Definition _tp : ident := $"tp".
 Definition _vec1 : ident := $"vec1".
 Definition _vec2 : ident := $"vec2".
@@ -246,7 +108,7 @@ Definition _t'5 : ident := 132%positive.
 
 Definition v_tasks := {|
   gvar_info := (tptr (Tstruct _task noattr));
-  gvar_init := (Init_space 4 :: nil);
+  gvar_init := (Init_space 8 :: nil);
   gvar_readonly := false;
   gvar_volatile := false
 |}.
@@ -260,7 +122,7 @@ Definition v_num_threads := {|
 
 Definition v_dtasks := {|
   gvar_info := (tptr (Tstruct _dotprod_task noattr));
-  gvar_init := (Init_space 4 :: nil);
+  gvar_init := (Init_space 8 :: nil);
   gvar_readonly := false;
   gvar_volatile := false
 |}.
@@ -271,9 +133,9 @@ Definition f_dotprod_worker := {|
   fn_params := ((_closure, (tptr tvoid)) :: nil);
   fn_vars := nil;
   fn_temps := ((_w, (tptr (Tstruct _dotprod_task noattr))) ::
-               (_result, tdouble) :: (_n, tuint) ::
+               (_result, tdouble) :: (_n, tulong) ::
                (_vec1, (tptr tdouble)) :: (_vec2, (tptr tdouble)) ::
-               (_i, tuint) :: (_t'2, tdouble) :: (_t'1, tdouble) :: nil);
+               (_i, tulong) :: (_t'2, tdouble) :: (_t'1, tdouble) :: nil);
   fn_body :=
 (Ssequence
   (Sset _w
@@ -285,7 +147,7 @@ Definition f_dotprod_worker := {|
       (Sset _n
         (Efield
           (Ederef (Etempvar _w (tptr (Tstruct _dotprod_task noattr)))
-            (Tstruct _dotprod_task noattr)) _n tuint))
+            (Tstruct _dotprod_task noattr)) _n tulong))
       (Ssequence
         (Sset _vec1
           (Efield
@@ -298,30 +160,30 @@ Definition f_dotprod_worker := {|
                 (Tstruct _dotprod_task noattr)) _vec2 (tptr tdouble)))
           (Ssequence
             (Ssequence
-              (Sset _i (Econst_int (Int.repr 0) tint))
+              (Sset _i (Ecast (Econst_int (Int.repr 0) tint) tulong))
               (Sloop
                 (Ssequence
-                  (Sifthenelse (Ebinop Olt (Etempvar _i tuint)
-                                 (Etempvar _n tuint) tint)
+                  (Sifthenelse (Ebinop Olt (Etempvar _i tulong)
+                                 (Etempvar _n tulong) tint)
                     Sskip
                     Sbreak)
                   (Ssequence
                     (Sset _t'1
                       (Ederef
                         (Ebinop Oadd (Etempvar _vec1 (tptr tdouble))
-                          (Etempvar _i tuint) (tptr tdouble)) tdouble))
+                          (Etempvar _i tulong) (tptr tdouble)) tdouble))
                     (Ssequence
                       (Sset _t'2
                         (Ederef
                           (Ebinop Oadd (Etempvar _vec2 (tptr tdouble))
-                            (Etempvar _i tuint) (tptr tdouble)) tdouble))
+                            (Etempvar _i tulong) (tptr tdouble)) tdouble))
                       (Sset _result
                         (Ebinop Oadd (Etempvar _result tdouble)
                           (Ebinop Omul (Etempvar _t'1 tdouble)
                             (Etempvar _t'2 tdouble) tdouble) tdouble)))))
                 (Sset _i
-                  (Ebinop Oadd (Etempvar _i tuint)
-                    (Econst_int (Int.repr 1) tint) tuint))))
+                  (Ebinop Oadd (Etempvar _i tulong)
+                    (Econst_int (Int.repr 1) tint) tulong))))
             (Sassign
               (Efield
                 (Ederef (Etempvar _w (tptr (Tstruct _dotprod_task noattr)))
@@ -333,12 +195,11 @@ Definition f_dotprod := {|
   fn_return := tdouble;
   fn_callconv := cc_default;
   fn_params := ((_vec1, (tptr tdouble)) :: (_vec2, (tptr tdouble)) ::
-                (_n, tuint) :: nil);
+                (_n, tulong) :: nil);
   fn_vars := nil;
   fn_temps := ((_result, tdouble) :: (_T, tuint) :: (_t, tuint) ::
-               (_delta, tuint) :: (_delta_next, tuint) ::
+               (_delta, tulong) :: (_delta_next, tulong) ::
                (_tp, (tptr (Tstruct _dotprod_task noattr))) ::
-               (_delta_next__1, tuint) ::
                (_t'4, (tptr (Tstruct _dotprod_task noattr))) ::
                (_t'3, (tptr (Tstruct _task noattr))) :: (_t'2, tdouble) ::
                (_t'1, (tptr (Tstruct _dotprod_task noattr))) :: nil);
@@ -346,7 +207,7 @@ Definition f_dotprod := {|
 (Ssequence
   (Sset _T (Evar _num_threads tuint))
   (Ssequence
-    (Sset _delta (Econst_int (Int.repr 0) tint))
+    (Sset _delta (Ecast (Econst_int (Int.repr 0) tint) tulong))
     (Ssequence
       (Ssequence
         (Sset _t (Econst_int (Int.repr 0) tint))
@@ -372,7 +233,7 @@ Definition f_dotprod := {|
                       (Etempvar _tp (tptr (Tstruct _dotprod_task noattr)))
                       (Tstruct _dotprod_task noattr)) _vec1 (tptr tdouble))
                   (Ebinop Oadd (Etempvar _vec1 (tptr tdouble))
-                    (Etempvar _delta tuint) (tptr tdouble)))
+                    (Etempvar _delta tulong) (tptr tdouble)))
                 (Ssequence
                   (Sassign
                     (Efield
@@ -380,26 +241,25 @@ Definition f_dotprod := {|
                         (Etempvar _tp (tptr (Tstruct _dotprod_task noattr)))
                         (Tstruct _dotprod_task noattr)) _vec2 (tptr tdouble))
                     (Ebinop Oadd (Etempvar _vec2 (tptr tdouble))
-                      (Etempvar _delta tuint) (tptr tdouble)))
+                      (Etempvar _delta tulong) (tptr tdouble)))
                   (Ssequence
-                    (Sset _delta_next__1
-                      (Ecast
-                        (Ebinop Odiv
-                          (Ebinop Omul
-                            (Ecast
-                              (Ebinop Oadd (Etempvar _t tuint)
-                                (Econst_int (Int.repr 1) tint) tuint) tulong)
-                            (Ecast (Etempvar _n tuint) tulong) tulong)
-                          (Ecast (Etempvar _T tuint) tulong) tulong) tuint))
+                    (Sset _delta_next
+                      (Ebinop Odiv
+                        (Ebinop Omul
+                          (Ecast
+                            (Ebinop Oadd (Etempvar _t tuint)
+                              (Econst_int (Int.repr 1) tint) tuint) tulong)
+                          (Ecast (Etempvar _n tulong) tulong) tulong)
+                        (Ecast (Etempvar _T tuint) tulong) tulong))
                     (Ssequence
                       (Sassign
                         (Efield
                           (Ederef
                             (Etempvar _tp (tptr (Tstruct _dotprod_task noattr)))
-                            (Tstruct _dotprod_task noattr)) _n tuint)
-                        (Ebinop Osub (Etempvar _delta_next__1 tuint)
-                          (Etempvar _delta tuint) tuint))
-                      (Sset _delta (Etempvar _delta_next__1 tuint))))))))
+                            (Tstruct _dotprod_task noattr)) _n tulong)
+                        (Ebinop Osub (Etempvar _delta_next tulong)
+                          (Etempvar _delta tulong) tulong))
+                      (Sset _delta (Etempvar _delta_next tulong))))))))
           (Sset _t
             (Ebinop Oadd (Etempvar _t tuint) (Econst_int (Int.repr 1) tint)
               tuint))))
@@ -469,10 +329,10 @@ Definition f_make_dotprod_tasks := {|
     (Ssequence
       (Ssequence
         (Scall (Some _t'2)
-          (Evar _malloc (Tfunction (Tcons tuint Tnil) (tptr tvoid)
+          (Evar _malloc (Tfunction (Tcons tulong Tnil) (tptr tvoid)
                           cc_default))
           ((Ebinop Omul (Etempvar _T tuint)
-             (Esizeof (Tstruct _dotprod_task noattr) tuint) tuint) :: nil))
+             (Esizeof (Tstruct _dotprod_task noattr) tulong) tulong) :: nil))
         (Sassign (Evar _dtasks (tptr (Tstruct _dotprod_task noattr)))
           (Ecast (Etempvar _t'2 (tptr tvoid))
             (tptr (Tstruct _dotprod_task noattr)))))
@@ -483,7 +343,8 @@ Definition f_make_dotprod_tasks := {|
                          (Etempvar _t'5 (tptr (Tstruct _dotprod_task noattr)))
                          tint)
             (Scall None
-              (Evar _exit (Tfunction (Tcons tint Tnil) tvoid cc_default))
+              (Evar _exit_thread (Tfunction (Tcons tint Tnil) tvoid
+                                   cc_default))
               ((Econst_int (Int.repr 1) tint) :: nil))
             Sskip))
         (Ssequence
@@ -529,26 +390,26 @@ Definition f_make_dotprod_tasks := {|
 Definition composites : list composite_definition :=
 (Composite _dotprod_task Struct
    (Member_plain _vec1 (tptr tdouble) :: Member_plain _vec2 (tptr tdouble) ::
-    Member_plain _n tuint :: Member_plain _result tdouble :: nil)
+    Member_plain _n tulong :: Member_plain _result tdouble :: nil)
    noattr :: nil).
 
 Definition global_definitions : list (ident * globdef fundef type) :=
 ((___compcert_va_int32,
    Gfun(External (EF_runtime "__compcert_va_int32"
-                   (mksignature (AST.Tint :: nil) AST.Tint cc_default))
+                   (mksignature (AST.Tlong :: nil) AST.Tint cc_default))
      (Tcons (tptr tvoid) Tnil) tuint cc_default)) ::
  (___compcert_va_int64,
    Gfun(External (EF_runtime "__compcert_va_int64"
-                   (mksignature (AST.Tint :: nil) AST.Tlong cc_default))
+                   (mksignature (AST.Tlong :: nil) AST.Tlong cc_default))
      (Tcons (tptr tvoid) Tnil) tulong cc_default)) ::
  (___compcert_va_float64,
    Gfun(External (EF_runtime "__compcert_va_float64"
-                   (mksignature (AST.Tint :: nil) AST.Tfloat cc_default))
+                   (mksignature (AST.Tlong :: nil) AST.Tfloat cc_default))
      (Tcons (tptr tvoid) Tnil) tdouble cc_default)) ::
  (___compcert_va_composite,
    Gfun(External (EF_runtime "__compcert_va_composite"
-                   (mksignature (AST.Tint :: AST.Tint :: nil) AST.Tint
-                     cc_default)) (Tcons (tptr tvoid) (Tcons tuint Tnil))
+                   (mksignature (AST.Tlong :: AST.Tlong :: nil) AST.Tlong
+                     cc_default)) (Tcons (tptr tvoid) (Tcons tulong Tnil))
      (tptr tvoid) cc_default)) ::
  (___compcert_i64_dtos,
    Gfun(External (EF_runtime "__compcert_i64_dtos"
@@ -641,8 +502,8 @@ Definition global_definitions : list (ident * globdef fundef type) :=
      (Tcons tuint Tnil) tint cc_default)) ::
  (___builtin_clzl,
    Gfun(External (EF_builtin "__builtin_clzl"
-                   (mksignature (AST.Tint :: nil) AST.Tint cc_default))
-     (Tcons tuint Tnil) tint cc_default)) ::
+                   (mksignature (AST.Tlong :: nil) AST.Tint cc_default))
+     (Tcons tulong Tnil) tint cc_default)) ::
  (___builtin_clzll,
    Gfun(External (EF_builtin "__builtin_clzll"
                    (mksignature (AST.Tlong :: nil) AST.Tint cc_default))
@@ -653,8 +514,8 @@ Definition global_definitions : list (ident * globdef fundef type) :=
      (Tcons tuint Tnil) tint cc_default)) ::
  (___builtin_ctzl,
    Gfun(External (EF_builtin "__builtin_ctzl"
-                   (mksignature (AST.Tint :: nil) AST.Tint cc_default))
-     (Tcons tuint Tnil) tint cc_default)) ::
+                   (mksignature (AST.Tlong :: nil) AST.Tint cc_default))
+     (Tcons tulong Tnil) tint cc_default)) ::
  (___builtin_ctzll,
    Gfun(External (EF_builtin "__builtin_ctzll"
                    (mksignature (AST.Tlong :: nil) AST.Tint cc_default))
@@ -678,10 +539,10 @@ Definition global_definitions : list (ident * globdef fundef type) :=
  (___builtin_memcpy_aligned,
    Gfun(External (EF_builtin "__builtin_memcpy_aligned"
                    (mksignature
-                     (AST.Tint :: AST.Tint :: AST.Tint :: AST.Tint :: nil)
-                     AST.Tvoid cc_default))
+                     (AST.Tlong :: AST.Tlong :: AST.Tlong :: AST.Tlong ::
+                      nil) AST.Tvoid cc_default))
      (Tcons (tptr tvoid)
-       (Tcons (tptr tvoid) (Tcons tuint (Tcons tuint Tnil)))) tvoid
+       (Tcons (tptr tvoid) (Tcons tulong (Tcons tulong Tnil)))) tvoid
      cc_default)) ::
  (___builtin_sel,
    Gfun(External (EF_builtin "__builtin_sel"
@@ -691,13 +552,13 @@ Definition global_definitions : list (ident * globdef fundef type) :=
      {|cc_vararg:=(Some 1); cc_unproto:=false; cc_structret:=false|})) ::
  (___builtin_annot,
    Gfun(External (EF_builtin "__builtin_annot"
-                   (mksignature (AST.Tint :: nil) AST.Tvoid
+                   (mksignature (AST.Tlong :: nil) AST.Tvoid
                      {|cc_vararg:=(Some 1); cc_unproto:=false; cc_structret:=false|}))
      (Tcons (tptr tschar) Tnil) tvoid
      {|cc_vararg:=(Some 1); cc_unproto:=false; cc_structret:=false|})) ::
  (___builtin_annot_intval,
    Gfun(External (EF_builtin "__builtin_annot_intval"
-                   (mksignature (AST.Tint :: AST.Tint :: nil) AST.Tint
+                   (mksignature (AST.Tlong :: AST.Tint :: nil) AST.Tint
                      cc_default)) (Tcons (tptr tschar) (Tcons tint Tnil))
      tint cc_default)) ::
  (___builtin_membar,
@@ -706,21 +567,21 @@ Definition global_definitions : list (ident * globdef fundef type) :=
      cc_default)) ::
  (___builtin_va_start,
    Gfun(External (EF_builtin "__builtin_va_start"
-                   (mksignature (AST.Tint :: nil) AST.Tvoid cc_default))
+                   (mksignature (AST.Tlong :: nil) AST.Tvoid cc_default))
      (Tcons (tptr tvoid) Tnil) tvoid cc_default)) ::
  (___builtin_va_arg,
    Gfun(External (EF_builtin "__builtin_va_arg"
-                   (mksignature (AST.Tint :: AST.Tint :: nil) AST.Tvoid
+                   (mksignature (AST.Tlong :: AST.Tint :: nil) AST.Tvoid
                      cc_default)) (Tcons (tptr tvoid) (Tcons tuint Tnil))
      tvoid cc_default)) ::
  (___builtin_va_copy,
    Gfun(External (EF_builtin "__builtin_va_copy"
-                   (mksignature (AST.Tint :: AST.Tint :: nil) AST.Tvoid
+                   (mksignature (AST.Tlong :: AST.Tlong :: nil) AST.Tvoid
                      cc_default))
      (Tcons (tptr tvoid) (Tcons (tptr tvoid) Tnil)) tvoid cc_default)) ::
  (___builtin_va_end,
    Gfun(External (EF_builtin "__builtin_va_end"
-                   (mksignature (AST.Tint :: nil) AST.Tvoid cc_default))
+                   (mksignature (AST.Tlong :: nil) AST.Tvoid cc_default))
      (Tcons (tptr tvoid) Tnil) tvoid cc_default)) ::
  (___builtin_unreachable,
    Gfun(External (EF_builtin "__builtin_unreachable"
@@ -728,8 +589,8 @@ Definition global_definitions : list (ident * globdef fundef type) :=
      cc_default)) ::
  (___builtin_expect,
    Gfun(External (EF_builtin "__builtin_expect"
-                   (mksignature (AST.Tint :: AST.Tint :: nil) AST.Tint
-                     cc_default)) (Tcons tint (Tcons tint Tnil)) tint
+                   (mksignature (AST.Tlong :: AST.Tlong :: nil) AST.Tlong
+                     cc_default)) (Tcons tlong (Tcons tlong Tnil)) tlong
      cc_default)) ::
  (___builtin_fmax,
    Gfun(External (EF_builtin "__builtin_fmax"
@@ -771,21 +632,21 @@ Definition global_definitions : list (ident * globdef fundef type) :=
      cc_default)) ::
  (___builtin_read16_reversed,
    Gfun(External (EF_builtin "__builtin_read16_reversed"
-                   (mksignature (AST.Tint :: nil) AST.Tint16unsigned
+                   (mksignature (AST.Tlong :: nil) AST.Tint16unsigned
                      cc_default)) (Tcons (tptr tushort) Tnil) tushort
      cc_default)) ::
  (___builtin_read32_reversed,
    Gfun(External (EF_builtin "__builtin_read32_reversed"
-                   (mksignature (AST.Tint :: nil) AST.Tint cc_default))
+                   (mksignature (AST.Tlong :: nil) AST.Tint cc_default))
      (Tcons (tptr tuint) Tnil) tuint cc_default)) ::
  (___builtin_write16_reversed,
    Gfun(External (EF_builtin "__builtin_write16_reversed"
-                   (mksignature (AST.Tint :: AST.Tint :: nil) AST.Tvoid
+                   (mksignature (AST.Tlong :: AST.Tint :: nil) AST.Tvoid
                      cc_default)) (Tcons (tptr tushort) (Tcons tushort Tnil))
      tvoid cc_default)) ::
  (___builtin_write32_reversed,
    Gfun(External (EF_builtin "__builtin_write32_reversed"
-                   (mksignature (AST.Tint :: AST.Tint :: nil) AST.Tvoid
+                   (mksignature (AST.Tlong :: AST.Tint :: nil) AST.Tvoid
                      cc_default)) (Tcons (tptr tuint) (Tcons tuint Tnil))
      tvoid cc_default)) ::
  (___builtin_debug,
@@ -794,20 +655,20 @@ Definition global_definitions : list (ident * globdef fundef type) :=
                      {|cc_vararg:=(Some 1); cc_unproto:=false; cc_structret:=false|}))
      (Tcons tint Tnil) tvoid
      {|cc_vararg:=(Some 1); cc_unproto:=false; cc_structret:=false|})) ::
- (_exit,
-   Gfun(External (EF_external "exit"
+ (_malloc,
+   Gfun(External EF_malloc (Tcons tulong Tnil) (tptr tvoid) cc_default)) ::
+ (_exit_thread,
+   Gfun(External (EF_external "exit_thread"
                    (mksignature (AST.Tint :: nil) AST.Tvoid cc_default))
      (Tcons tint Tnil) tvoid cc_default)) ::
- (_malloc,
-   Gfun(External EF_malloc (Tcons tuint Tnil) (tptr tvoid) cc_default)) ::
  (_make_tasks,
    Gfun(External (EF_external "make_tasks"
-                   (mksignature (AST.Tint :: nil) AST.Tint cc_default))
+                   (mksignature (AST.Tint :: nil) AST.Tlong cc_default))
      (Tcons tuint Tnil) (tptr (Tstruct _task noattr)) cc_default)) ::
  (_initialize_task,
    Gfun(External (EF_external "initialize_task"
                    (mksignature
-                     (AST.Tint :: AST.Tint :: AST.Tint :: AST.Tint :: nil)
+                     (AST.Tlong :: AST.Tint :: AST.Tlong :: AST.Tlong :: nil)
                      AST.Tvoid cc_default))
      (Tcons (tptr (Tstruct _task noattr))
        (Tcons tuint
@@ -815,7 +676,7 @@ Definition global_definitions : list (ident * globdef fundef type) :=
            (Tcons (tptr tvoid) Tnil)))) tvoid cc_default)) ::
  (_do_tasks,
    Gfun(External (EF_external "do_tasks"
-                   (mksignature (AST.Tint :: AST.Tint :: nil) AST.Tvoid
+                   (mksignature (AST.Tlong :: AST.Tint :: nil) AST.Tvoid
                      cc_default))
      (Tcons (tptr (Tstruct _task noattr)) (Tcons tuint Tnil)) tvoid
      cc_default)) :: (_tasks, Gvar v_tasks) ::
@@ -827,26 +688,26 @@ Definition global_definitions : list (ident * globdef fundef type) :=
 Definition public_idents : list ident :=
 (_make_dotprod_tasks :: _dotprod :: _dotprod_worker :: _dtasks ::
  _num_threads :: _tasks :: _do_tasks :: _initialize_task :: _make_tasks ::
- _malloc :: _exit :: ___builtin_debug :: ___builtin_write32_reversed ::
- ___builtin_write16_reversed :: ___builtin_read32_reversed ::
- ___builtin_read16_reversed :: ___builtin_fnmsub :: ___builtin_fnmadd ::
- ___builtin_fmsub :: ___builtin_fmadd :: ___builtin_fmin ::
- ___builtin_fmax :: ___builtin_expect :: ___builtin_unreachable ::
- ___builtin_va_end :: ___builtin_va_copy :: ___builtin_va_arg ::
- ___builtin_va_start :: ___builtin_membar :: ___builtin_annot_intval ::
- ___builtin_annot :: ___builtin_sel :: ___builtin_memcpy_aligned ::
- ___builtin_sqrt :: ___builtin_fsqrt :: ___builtin_fabsf ::
- ___builtin_fabs :: ___builtin_ctzll :: ___builtin_ctzl :: ___builtin_ctz ::
- ___builtin_clzll :: ___builtin_clzl :: ___builtin_clz ::
- ___builtin_bswap16 :: ___builtin_bswap32 :: ___builtin_bswap ::
- ___builtin_bswap64 :: ___compcert_i64_umulh :: ___compcert_i64_smulh ::
- ___compcert_i64_sar :: ___compcert_i64_shr :: ___compcert_i64_shl ::
- ___compcert_i64_umod :: ___compcert_i64_smod :: ___compcert_i64_udiv ::
- ___compcert_i64_sdiv :: ___compcert_i64_utof :: ___compcert_i64_stof ::
- ___compcert_i64_utod :: ___compcert_i64_stod :: ___compcert_i64_dtou ::
- ___compcert_i64_dtos :: ___compcert_va_composite ::
- ___compcert_va_float64 :: ___compcert_va_int64 :: ___compcert_va_int32 ::
- nil).
+ _exit_thread :: _malloc :: ___builtin_debug ::
+ ___builtin_write32_reversed :: ___builtin_write16_reversed ::
+ ___builtin_read32_reversed :: ___builtin_read16_reversed ::
+ ___builtin_fnmsub :: ___builtin_fnmadd :: ___builtin_fmsub ::
+ ___builtin_fmadd :: ___builtin_fmin :: ___builtin_fmax ::
+ ___builtin_expect :: ___builtin_unreachable :: ___builtin_va_end ::
+ ___builtin_va_copy :: ___builtin_va_arg :: ___builtin_va_start ::
+ ___builtin_membar :: ___builtin_annot_intval :: ___builtin_annot ::
+ ___builtin_sel :: ___builtin_memcpy_aligned :: ___builtin_sqrt ::
+ ___builtin_fsqrt :: ___builtin_fabsf :: ___builtin_fabs ::
+ ___builtin_ctzll :: ___builtin_ctzl :: ___builtin_ctz :: ___builtin_clzll ::
+ ___builtin_clzl :: ___builtin_clz :: ___builtin_bswap16 ::
+ ___builtin_bswap32 :: ___builtin_bswap :: ___builtin_bswap64 ::
+ ___compcert_i64_umulh :: ___compcert_i64_smulh :: ___compcert_i64_sar ::
+ ___compcert_i64_shr :: ___compcert_i64_shl :: ___compcert_i64_umod ::
+ ___compcert_i64_smod :: ___compcert_i64_udiv :: ___compcert_i64_sdiv ::
+ ___compcert_i64_utof :: ___compcert_i64_stof :: ___compcert_i64_utod ::
+ ___compcert_i64_stod :: ___compcert_i64_dtou :: ___compcert_i64_dtos ::
+ ___compcert_va_composite :: ___compcert_va_float64 ::
+ ___compcert_va_int64 :: ___compcert_va_int32 :: nil).
 
 Definition prog : Clight.program := 
   mkprogram composites global_definitions public_idents _main Logic.I.
